proof/spec/Utils.ec
@@ -5,3 +5,14 @@ require import BitEncoding.
 (*---*) import BitChunking.
 
 from Jasmin require import JModel.
+
+module Utils = {
+  proc w64_to_bytes (x : W64.t, outlen : int) = {
+    var r : W8.t list;
+    
+    (* TODO: FIX THIS *)
+    r <- nseq outlen W8.zero;
+  
+    return r;
+  } 
+}.
