proof/correctness/Repr.ec
@@ -3,20 +3,15 @@ pragma Goals : printall.
 require import AllCore List.
 from Jasmin require import JModel.
 
-require import Address Wots XMSS_MT_PRF.
-require import XMSS_IMPL XMSS_IMPL_PP.
+require import Address Notation Primitives Wots XMSS_MT_PRF.
+require import RandomBytes XMSS_IMPL.
 
-require import Array32 Array2144.
+require import Array32 Array64 Array2144.
 
-(* 
-    Operators to convert impl representation (i.e. arrays) to spec representation and
-    predicates for equality 
+require import BitEncoding.
+(*---*) import BitChunking.
 
-    Enc :: Spec -> Impl
-    Dec :: Impl -> Spec
-    
-    Dec . Enc = Id
-*)
+(*---*) import NBytes.
 
 (**************************************************************************************************)
 (*******************                        MEM                                 *******************)
@@ -36,29 +31,32 @@ rewrite /load_mem_w8_list32 /load_mem_w8_array32.
 apply (eq_from_nth witness) ; [ rewrite /to_list !size_mkseq //= | smt(@List @Array32) ].
 qed.
 
-
-(**************************************************************************************************)
-(*******************                        HASH                                *******************)
-(**************************************************************************************************)
-
-
 (**************************************************************************************************)
 (*******************                        WOTS                                *******************)
 (**************************************************************************************************)
 
-op enc_wots_sk (sk : wots_sk) : W8.t Array2144.t =
-    Array2144.of_list witness (flatten sk).
+(* Encode : impl -> spec *)
+(* Decode : spec -> impl *)
 
+op EncodeWotsMessage (m : W8.t Array32.t) : nbytes = to_list m.
+op EncodeWotsMsgBaseW (m : W8.t Array64.t) : W8.t list = to_list m.
+op EncodeWotsSignature (s : W8.t Array2144.t) : wots_signature = chunk 32 (to_list s). (* cada chunk tem nbytes /\ n = 32 *)
+op EncodeWotsPk (pk : W8.t Array2144.t) : wots_pk = chunk 32 (to_list pk).
+op EncodeWotsSk (sk : W8.t Array2144.t) : wots_sk = chunk 32 (to_list sk).
 
-pred eq_wots_sk (sk_impl : W8.t Array2144.t) (sk_spec : wots_sk) = 
-    flatten sk_spec = (to_list sk_impl).
+op DecodeWotsMessage (m : wots_message) : W8.t Array32.t = Array32.of_list witness m.
+op DecodeWotsMsgBaseW (m : wots_message_base_w) : W8.t Array64.t = Array64.of_list witness m.
+op DecodeWotsSignature (s : wots_signature) : W8.t Array2144.t = Array2144.of_list witness (flatten s).
+op DecodeWotsPk (pk : wots_pk) : W8.t Array2144.t = Array2144.of_list witness (flatten pk).
+op DecodeWotsSk (sk : wots_sk) : W8.t Array2144.t = Array2144.of_list witness (flatten sk).
 
-op enc_wots_pk (pk : wots_pk) : W8.t Array2144.t =
-    Array2144.of_list witness (flatten pk).
+(*-------------------------------------------------------------------------------------------------*)
 
+op sig_from_ptr_array (mem : global_mem_t) (ptr : W64.t) : W8.t Array2144.t =     
+  Array2144.init (fun (i : int) => loadW8 mem (to_uint ptr + i)).
 
-pred eq_wots_pk (pk_impl : W8.t Array2144.t) (pk_spec : wots_pk) = 
-    flatten pk_spec = (to_list pk_impl).
+op sig_from_ptr_list (mem : global_mem_t) (ptr : W64.t) : W8.t list =     
+  mkseq (fun (i : int) => loadW8 mem (to_uint ptr + i)) 2144.
 
 (**************************************************************************************************)
 (*******************                        XNSS                                *******************)
