proof/spec/Hash.ec
@@ -1,0 +1,55 @@
+pragma Goals : printall.
+
+require import AllCore List Distr RealExp IntDiv.
+require import BitEncoding.
+(*---*) import BitChunking.
+
+from Jasmin require import JModel.
+
+require import Primitives.
+
+(*---*) import NBytes.
+
+op Hash : W8.t list -> W8.t list.
+
+op prf_padding_val : W64.t.
+op prf_kg_padding_val : W64.t.
+op padding_len : int.
+
+module Hash = {
+  proc w64_to_bytes (x :W64.t, outlen : int) : W8.t list = { (* TODO: Move to Utils *)
+    var r : W8.t list;
+
+    r <- nseq outlen W8.zero;
+
+    return r;
+  }
+
+  proc prf (in_0 : W8.t list, key : nbytes) : nbytes = {
+    var r : nbytes;
+    var padding : W8.t list;
+    var buf : W8.t list;
+
+    padding <@ w64_to_bytes (prf_padding_val, padding_len);
+    buf <- padding ++ key ++ in_0;
+
+    r <- Hash buf;
+
+    return r;
+  }
+
+
+  proc prf_keygen (in_0 : W8.t list, key : nbytes) : nbytes = {
+    var r : nbytes;
+    var padding : W8.t list;
+    var buf : W8.t list;
+
+    padding <@ w64_to_bytes (prf_kg_padding_val, padding_len);
+    buf <- padding ++ key ++ in_0;
+
+    r <- Hash buf;
+    
+    return r;
+
+  }
+}.
